cedar-lean/Cedar/Thm/TPE/WellTyped/Set.lean
@@ -41,7 +41,7 @@ theorem partial_eval_well_typed_set {env : TypeEnv} {ls : List Residual} {ty : C
   intros h_ls_wt h_wf h_ref h_wt
   cases h_wt
   rename_i ty₁ h₀ h₁ h₂
-  simp only [TPE.evaluate, TPE.set, List.any_eq_true]
+  simp only [TPE.evaluate, TPE.set]
   split
   case h_1 x xs h₃ =>
     apply Residual.WellTyped.val
@@ -75,8 +75,7 @@ theorem partial_eval_well_typed_set {env : TypeEnv} {ls : List Residual} {ty : C
   case h_2 x h₃ =>
     split
     . apply Residual.WellTyped.error
-    case isFalse _ =>
-      apply Residual.WellTyped.set
+    · apply Residual.WellTyped.set
       . intro x h₅
         simp only [List.map₁, List.attach, List.map_subtype, List.unattach_attachWith, List.mem_map] at h₅
         rcases h₅ with ⟨x₂, h₆, h₇⟩
